Remove unIdent (#627)

cava/Cava/Acorn/Identity.v
@@ -14,58 +14,19 @@
 (* limitations under the License.                                           *)
 (****************************************************************************)
 
-Require Import Coq.Lists.List.
 Require Import Coq.Vectors.Vector.
-Require Import Coq.micromega.Lia.
-Require Import coqutil.Tactics.Tactics.
+Require Import ExtLib.Data.List.
+Require Import ExtLib.Data.Vector.
 Require Import ExtLib.Structures.Monad.
 Require Import ExtLib.Structures.MonadLaws.
-Require Import Cava.Signal.
-Require Import Cava.Tactics.
-Require Import Cava.ListUtils.
+Require Import ExtLib.Structures.Traversable.
 Require Import Cava.VectorUtils.
-Require Import Cava.Lib.BitVectorOps.
-Require Import Cava.Acorn.CavaClass.
-Require Import Cava.Acorn.Combinational.
-Require Import Cava.Acorn.Combinators.
-Import VectorNotations ListNotations.
-Open Scope list_scope.
 
-Existing Instance CombinationalSemantics.
-
-Section MapT.
-  Lemma mapT_vector_ident {A B n} (f : A -> ident B) (v : Vector.t A n) :
-    unIdent (mapT_vector f v) = map (fun a => unIdent (f a)) v.
-  Proof.
-    induction v; intros; [ reflexivity | ].
-    cbn. rewrite IHv. reflexivity.
-  Qed.
-  (* Alternate form of the above with the Traversable wrapper not simplified *)
-  Lemma mapT_vident {A B n} (f : A -> ident B) (v : Vector.t A n) :
-    unIdent (Traversable.mapT
-               (Traversable:=Traversable_vector)
-               f v) = map (fun a => unIdent (f a)) v.
-  Proof. apply mapT_vector_ident. Qed.
-
-  Lemma mapT_lident {A B} (f : A -> ident B) (l : list A) :
-    unIdent (Traversable.mapT
-               (Traversable:=List.Traversable_list)
-               f l) = List.map (fun a => unIdent (f a)) l.
-  Proof.
-    simpl. induction l; [ reflexivity | ].
-    simpl. rewrite IHl. reflexivity.
-  Qed.
-End MapT.
+(* Identity monad *)
+Definition ident (T : Type) := T.
+Instance Monad_ident : Monad ident :=
+  { ret := fun _ t => t;
+    bind := fun _ _ x f => f x }.
 
 Instance MonadLaws_ident : MonadLaws Monad_ident.
 Proof. econstructor; intros; exact eq_refl. Defined.
-
-(* Automation to help simplify expressions using the identity monad *)
-Create HintDb simpl_ident discriminated.
-Hint Rewrite @mapT_vector_ident @mapT_vident @mapT_lident using solve [eauto] : simpl_ident.
-Ltac simpl_ident :=
-  repeat
-    first [ progress autorewrite with simpl_ident
-          | progress cbn [fst snd bind ret Monad_ident monad
-                              unpackV packV constant
-                              CombinationalSemantics unIdent] ].
