cava/Cava/Lib/UnsignedAdderProofs.v
@@ -20,7 +20,6 @@ Import ListNotations.
 Require Import Coq.Vectors.Vector.
 Import VectorNotations.
 Require Import ExtLib.Structures.Monads.
-Require Export ExtLib.Data.Monads.IdentityMonad.
 Require Import ExtLib.Structures.MonadLaws.
 Import MonadNotation.
 Open Scope monad_scope.
@@ -40,7 +39,7 @@ Local Open Scope N_scope.
 (* First prove the full-adder correct. *)
 
 Lemma fullAdder_correct (cin a b : bool) :
-  unIdent (fullAdder (cin, (a, b))) =
+  fullAdder (cin, (a, b)) =
   let sum := N.b2n a + N.b2n b + N.b2n cin in
   (N.testbit sum 0, N.testbit sum 1).
 Proof. destruct cin, a, b; reflexivity. Qed.
@@ -65,7 +64,7 @@ Hint Rewrite @bind_of_return @bind_associativity
 (* Correctness of the list based adder. *)
 Lemma addLCorrect (cin : bool) (a b : list bool) :
   length a = length b ->
-  list_bits_to_nat (unIdent (addLWithCinL cin a b)) =
+  list_bits_to_nat (addLWithCinL cin a b) =
   list_bits_to_nat a + list_bits_to_nat b + N.b2n cin.
 Proof.
   cbv zeta. cbv [addLWithCinL adderWithGrowthL unsignedAdderL colL].
@@ -89,7 +88,7 @@ Proof.
 
   (* Rearrange to match inductive hypothesis *)
   rewrite <-app_comm_cons.
-  cbn [unIdent] in *. rewrite list_bits_to_nat_cons.
+  rewrite list_bits_to_nat_cons.
 
   (* Finally we have the right expression to use IHa *)
   rewrite IHa by lia.
@@ -144,7 +143,7 @@ Proof.
 Qed.
 
 Lemma colL_length {A B C} circuit a bs :
-  length (fst (unIdent (@colL ident _ A B C circuit (a,bs))))
+  length (fst (@colL ident _ A B C circuit (a,bs)))
   = length bs.
 Proof.
   cbv [colL]; cbn [fst snd].
@@ -157,7 +156,7 @@ Qed.
 Hint Rewrite @colL_length using solve [length_hammer] : push_length.
 
 Lemma addVCorrect (cin : bool) (n : nat) (a b : Vector.t bool n) :
-  unIdent (addLWithCinV cin a b) =
+  addLWithCinV cin a b =
   (N2Bv_sized (n+1) (Bv2N a + Bv2N b + (N.b2n cin))).
 Proof.
   apply Bv2N_inj. rewrite Bv2N_N2Bv_sized.
