cava/Cava/Lib/VecProperties.v
@@ -29,72 +29,72 @@ Existing Instance CombinationalSemantics.
 Local Ltac crush :=
   (* inline Vec definition *)
   lazymatch goal with
-  | |- unIdent ?x = _ =>
+  | |- ?x = _ =>
     let f := app_head x in cbv [f]
   end;
-  simpl_ident; eauto using map_id_ext.
+  simpl_ident; eauto.
 
 
 Lemma bitvec_literal_correct n (v : Vector.t bool n) :
-  unIdent (Vec.bitvec_literal v) = v.
-Proof. crush. Qed.
+  Vec.bitvec_literal v = v.
+Proof. crush. apply map_id_ext; eauto. Qed.
 Hint Rewrite @bitvec_literal_correct using solve [eauto] : simpl_ident.
 
 Lemma nil_correct A :
-  unIdent (@Vec.nil _ _ A) = [].
+  @Vec.nil _ _ A = [].
 Proof. crush. Qed.
 Hint Rewrite @nil_correct using solve [eauto] : simpl_ident.
 
 Lemma cons_correct A n x (v : combType (Vec A n)) :
-  unIdent (Vec.cons x v) = (x :: v).
+  Vec.cons x v = (x :: v).
 Proof. crush. Qed.
 Hint Rewrite @cons_correct using solve [eauto] : simpl_ident.
 
 Lemma tl_correct A n (v : combType (Vec A (S n))) :
-  unIdent (Vec.tl v) = Vector.tl v.
+  Vec.tl v = Vector.tl v.
 Proof. crush. Qed.
 Hint Rewrite @tl_correct using solve [eauto] : simpl_ident.
 
 Lemma hd_correct A n (v : combType (Vec A (S n))) :
-  unIdent (Vec.hd v) = Vector.hd v.
+  Vec.hd v = Vector.hd v.
 Proof. crush. Qed.
 Hint Rewrite @hd_correct using solve [eauto] : simpl_ident.
 
 Lemma const_correct A (x : combType A) n :
-  unIdent (Vec.const x n) = Vector.const x n.
+  Vec.const x n = Vector.const x n.
 Proof. crush. Qed.
 Hint Rewrite @const_correct using solve [eauto] : simpl_ident.
 
 Lemma rev_correct A n (v : combType (Vec A (S n))) :
-  unIdent (Vec.rev v) = Vector.rev v.
+  Vec.rev v = Vector.rev v.
 Proof. crush. Qed.
 Hint Rewrite @rev_correct using solve [eauto] : simpl_ident.
 
 Lemma last_correct A n (v : combType (Vec A (S n))) :
-  unIdent (Vec.last v) = Vector.last v.
+  Vec.last v = Vector.last v.
 Proof. crush. Qed.
 Hint Rewrite @last_correct using solve [eauto] : simpl_ident.
 
 Lemma shiftin_correct A n x (v : combType (Vec A n)) :
-  unIdent (Vec.shiftin x v) = (Vector.shiftin x v).
+  Vec.shiftin x v = (Vector.shiftin x v).
 Proof. crush. Qed.
 Hint Rewrite @shiftin_correct using solve [eauto] : simpl_ident.
 
 Lemma shiftout_correct A n (v : combType (Vec A (S n))) :
-  unIdent (Vec.shiftout v) = Vector.shiftout v.
+  Vec.shiftout v = Vector.shiftout v.
 Proof. crush. Qed.
 Hint Rewrite @shiftout_correct using solve [eauto] : simpl_ident.
 
 Lemma transpose_correct A n m (v : combType (Vec (Vec A n) m)) :
-  unIdent (Vec.transpose v) = transpose v.
+  Vec.transpose v = transpose v.
 Proof.
   crush. rewrite !Vector.map_id; reflexivity.
 Qed.
 Hint Rewrite @transpose_correct using solve [eauto] : simpl_ident.
 
 Lemma fold_left_correct A B n f b v :
-  unIdent (@Vec.fold_left _ _ A B f n v b)
-  = Vector.fold_left (fun x y => unIdent (f (x,y))) b v.
+  @Vec.fold_left _ _ A B f n v b
+  = Vector.fold_left (fun x y => f (x,y)) b v.
 Proof.
   revert v b; induction n; intros;
     [ apply Vector.case0 with (v:=v); reflexivity | ].
@@ -106,8 +106,8 @@ Qed.
 Hint Rewrite @fold_left_correct using solve [eauto] : simpl_ident.
 
 Lemma fold_left2_correct A B C n f c va vb :
-  unIdent (@Vec.fold_left2 _ _ A B C f n va vb c)
-  = Vector.fold_left2 (fun x y z => unIdent (f (x,y,z))) c va vb.
+  @Vec.fold_left2 _ _ A B C f n va vb c
+  = Vector.fold_left2 (fun x y z => f (x,y,z)) c va vb.
 Proof.
   revert va vb c; induction n; intros;
     [ apply Vector.case0 with (v:=va);
@@ -121,14 +121,13 @@ Qed.
 Hint Rewrite @fold_left2_correct using solve [eauto] : simpl_ident.
 
 Lemma map_correct A B n f v :
-  unIdent (@Vec.map _ _ A B n f v)
-  = Vector.map (fun x => unIdent (f x)) v.
+  @Vec.map _ _ A B n f v = Vector.map f v.
 Proof. crush. Qed.
 Hint Rewrite @map_correct using solve [eauto] : simpl_ident.
 
 Lemma map2_correct A B C n f va vb :
-  unIdent (@Vec.map2 _ _ A B C n f va vb)
-  = Vector.map2 (fun x y => unIdent (f (x,y))) va vb.
+  @Vec.map2 _ _ A B C n f va vb
+  = Vector.map2 (fun x y => f (x,y)) va vb.
 Proof.
   crush. rewrite map_vcombine_map2.
   reflexivity.
