tests/TestMultiply.v
@@ -46,11 +46,11 @@ Definition bv3_7  := N2Bv_sized 3  7.
 Definition bv5_15 := N2Bv_sized 5 15.
 
 (* Check 3 * 5 = 30 *)
-Example mult3_5 : unIdent (multiplier (bv2_3, bv3_5)) = bv5_15.
+Example mult3_5 : multiplier (bv2_3, bv3_5) = bv5_15.
 Proof. reflexivity. Qed.
 
 (* Check 3 * 5 = 30 *)
-Example mult3_5_top : unIdent (multiplier (bv2_3, bv3_5)) = bv5_15.
+Example mult3_5_top : multiplier (bv2_3, bv3_5) = bv5_15.
 Proof. reflexivity. Qed.
 
 (******************************************************************************)
